Demo-Worthy Bookstore.

ADTExamples/QueryStructure/GeneralQueryRefinements.v
@@ -5,63 +5,83 @@ Require Import String Omega List FunctionalExtensionality Ensembles
 Definition Equivalent_Ensembles {A : Type}
            (P Q : Ensemble A) := forall a, P a <-> Q a.
 
-  Lemma Equivalent_Swap_In {A}
-        (qs : QueryStructureHint) (R R' : _)
-        (bod : Tuple -> Tuple -> Ensemble A)
-  :
-    Equivalent_Ensembles
-      (@Query_In qs _ R (fun tup => @Query_In qs _ R' (bod tup)))
-      (@Query_In qs _ R' (fun tup => @Query_In qs _ R
-                                               (fun tup' => bod tup' tup))).
-  Proof.
-    unfold Equivalent_Ensembles, Query_In; split; intros;
-    repeat (progress (destruct_ex; intuition)); eexists;
-    split; eauto.
-  Qed.
+Lemma Equivalent_Swap_In {A}
+      (qs : QueryStructureHint) (R R' : _)
+      (bod : Tuple -> Tuple -> Ensemble A)
+:
+  Equivalent_Ensembles
+    (@Query_In qs _ R (fun tup => @Query_In qs _ R' (bod tup)))
+    (@Query_In qs _ R' (fun tup => @Query_In qs _ R
+                                             (fun tup' => bod tup' tup))).
+Proof.
+  unfold Equivalent_Ensembles, Query_In; split; intros;
+  repeat (progress (destruct_ex; intuition)); eexists;
+  split; eauto.
+Qed.
 
-  Lemma Equivalent_Swap_In_Where {A}
-        (qs : QueryStructureHint) (R : _)
-        {heading}
-        (bod : @Tuple heading -> Tuple -> Ensemble A)
-        (P : @Tuple heading -> Prop)
-  :
-    pointwise_relation
-      Tuple Equivalent_Ensembles
-      (fun tup' : Tuple =>
-         (@Query_In qs _ R
-                    (fun tup => Query_Where (P tup') (bod tup' tup))))
-      (fun tup' : Tuple =>
-         Query_Where (P tup') (@Query_In qs _ R (bod tup'))).
-  Proof.
-    unfold Equivalent_Ensembles, Query_In, Query_Where; split; intros;
-    repeat (progress (destruct_ex; intuition)); eexists;
-    split; eauto.
-  Qed.
-
-  Add Parametric Morphism {A: Type} :
-    (Query_For)
-      with signature (@Equivalent_Ensembles A ==> refine)
-        as refine_Query_For_Equivalent.
-  Proof.
-    unfold impl, Query_For, refine; intros.
-    inversion_by computes_to_inv.
-    econstructor; split_iff; split; intros; eauto.
-    apply H; apply H1; auto.
-    apply H2; apply H; auto.
-  Qed.
-
-  Add Parametric Morphism {A: Type}
+Lemma Equivalent_Swap_In_Where {A}
       (qs : QueryStructureHint) (R : _)
-  :
-    (fun bod => Query_For (@Query_In qs _ R bod))
-      with signature ((pointwise_relation Tuple (@Equivalent_Ensembles A) ==> refine ))
-        as refine_Query_For_In_Equivalent.
-  Proof.
-    unfold impl, Query_For, pointwise_relation, Query_In, In, refine.
-    intros; inversion_by computes_to_inv.
-    econstructor; split_iff; split; intros; eauto.
-    destruct (H1 _ H0); eexists; intuition; eauto.
-    apply H; auto.
-    destruct_ex; apply H2; eexists; intuition; eauto.
-    apply H; auto.
-  Qed.
+      {heading}
+      (bod : @Tuple heading -> Tuple -> Ensemble A)
+      (P : @Tuple heading -> Prop)
+:
+  pointwise_relation
+    Tuple Equivalent_Ensembles
+    (fun tup' : Tuple =>
+       (@Query_In qs _ R
+                  (fun tup => Query_Where (P tup') (bod tup' tup))))
+    (fun tup' : Tuple =>
+       Query_Where (P tup') (@Query_In qs _ R (bod tup'))).
+Proof.
+  unfold Equivalent_Ensembles, Query_In, Query_Where; split; intros;
+  repeat (progress (destruct_ex; intuition)); eexists;
+  split; eauto.
+Qed.
+
+Add Parametric Morphism {A: Type} :
+  (Query_For)
+    with signature (@Equivalent_Ensembles A ==> refine)
+      as refine_Query_For_Equivalent.
+Proof.
+  unfold impl, Query_For, refine; intros.
+  inversion_by computes_to_inv.
+  econstructor; split_iff; split; intros; eauto.
+  apply H; apply H1; auto.
+  apply H2; apply H; auto.
+Qed.
+
+Add Parametric Morphism {A: Type}
+    (qs : QueryStructureHint) (R : _)
+:
+  (fun bod => Query_For (@Query_In qs _ R bod))
+    with signature ((pointwise_relation Tuple (@Equivalent_Ensembles A) ==> refine ))
+      as refine_Query_For_In_Equivalent.
+Proof.
+  unfold impl, Query_For, pointwise_relation, Query_In, In, refine.
+  intros; inversion_by computes_to_inv.
+  econstructor; split_iff; split; intros; eauto.
+  destruct (H1 _ H0); eexists; intuition; eauto.
+  apply H; auto.
+  destruct_ex; apply H2; eexists; intuition; eauto.
+  apply H; auto.
+Qed.
+
+Class DecideableWhereClause {A} (P : Ensemble A) :=
+  { cond : A -> bool;
+    cond_dec : forall a, cond a = true <-> P a}.
+
+Instance DecideableWhereClause_EqString {A : Type}
+         (f f' : A -> string)
+         : DecideableWhereClause (fun a => eq (f a) (f' a)) :=
+  {| cond a := if string_dec (f a) (f' a) then true else false |}.
+Proof.
+  intros; find_if_inside; split; congruence.
+Defined.
+
+Instance DecideableWhereClause_EqNat {A : Type}
+         (f f' : A -> nat)
+         : DecideableWhereClause (fun a => eq (f a) (f' a)) :=
+  {| cond a := if eq_nat_dec (f a) (f' a) then true else false |}.
+Proof.
+  intros; find_if_inside; split; congruence.
+Defined.
