ADTExamples/QueryStructure/GeneralInsertRefinements.v
@@ -7,19 +7,57 @@ Lemma tupleAgree_refl :
          (tup : @Tuple h)
          (attrlist : list (Attributes h)),
     tupleAgree tup tup attrlist.
-  Proof.
-    unfold tupleAgree; auto.
-  Qed.
+Proof.
+  unfold tupleAgree; auto.
+Qed.
 
-  Lemma refine_tupleAgree_refl_True :
-    forall (h : Heading)
-           (tup : @Tuple h)
-           (attrlist attrlist' : list (Attributes h)),
-      refine {b |
-              decides b (tupleAgree tup tup attrlist'
-                         -> tupleAgree tup tup attrlist)}
-             (ret true).
-  Proof.
-    unfold refine; intros; inversion_by computes_to_inv.
-    subst; econstructor; simpl; auto using tupleAgree_refl.
-  Qed.
+Lemma refine_tupleAgree_refl_True :
+  forall (h : Heading)
+         (tup : @Tuple h)
+         (attrlist attrlist' : list (Attributes h)),
+    refine {b |
+            decides b (tupleAgree tup tup attrlist'
+                       -> tupleAgree tup tup attrlist)}
+           (ret true).
+Proof.
+  unfold refine; intros; inversion_by computes_to_inv.
+  subst; econstructor; simpl; auto using tupleAgree_refl.
+Qed.
+
+Ltac simplify_trivial_SatisfiesSchemaConstraints :=
+  simpl;
+  try rewrite refine_tupleAgree_refl_True;
+  try setoid_rewrite decides_True;
+  try setoid_rewrite decides_2_True; reflexivity.
+
+Ltac simplify_trivial_SatisfiesCrossRelationConstraints :=
+  simpl; try setoid_rewrite decides_True;
+  try setoid_rewrite decides_3_True;
+  repeat setoid_rewrite refineEquiv_bind_unit;
+  unfold If_Then_Else;
+  try setoid_rewrite refine_if_bool_eta; reflexivity.
+
+Tactic Notation "remove" "trivial" "insertion" "checks" :=
+  intros; setoid_rewrite QSInsertSpec_UnConstr_refine; eauto;
+  [ | simplify_trivial_SatisfiesSchemaConstraints
+    | simplify_trivial_SatisfiesSchemaConstraints
+    | simplify_trivial_SatisfiesSchemaConstraints
+    | simplify_trivial_SatisfiesCrossRelationConstraints
+    | simplify_trivial_SatisfiesCrossRelationConstraints ];
+  repeat setoid_rewrite refineEquiv_bind_unit;
+  repeat setoid_rewrite refineEquiv_bind_bind;
+  repeat setoid_rewrite refineEquiv_bind_unit.
+
+Tactic Notation "Split" "Constraint" "Checks" :=
+  let b := match goal with
+             | [ |- context[if ?X then _ else _] ] => constr:(X)
+             | [ H : context[if ?X then _ else _] |- _ ]=> constr:(X)
+           end in
+  let b_eq := fresh in
+  eapply (@refine_if _ _ b); intros b_eq;
+  repeat setoid_rewrite b_eq;
+  repeat rewrite b_eq.
+
+Tactic Notation "implement" "failed" "insert" :=
+  repeat (rewrite refine_pick_val, refineEquiv_bind_unit; eauto);
+  reflexivity.
