ADTExamples/QueryStructure/ListInsertRefinements.v
@@ -1,96 +1,151 @@
 Require Import String Omega List FunctionalExtensionality Ensembles
         Computation ADT ADTRefinement ADTNotation QueryStructureSchema
-        QueryQSSpecs InsertQSSpecs QueryStructure ProcessScheduler.AdditionalLemmas.
+        QueryQSSpecs InsertQSSpecs QueryStructure
+        ProcessScheduler.AdditionalLemmas GeneralQueryRefinements.
 
 Definition decideable_Heading_Domain
-             (h : Heading) :=
-    forall (idx : Attributes h)
-           (t t' : Domain h idx), {t = t'} + {t <> t'}.
+           (h : Heading) :=
+  forall (idx : Attributes h)
+         (t t' : Domain h idx), {t = t'} + {t <> t'}.
 
-  Fixpoint Tuple_Agree_dec
-             (h : Heading)
-             (h_dec_eq : decideable_Heading_Domain h)
-             (attrlist : list (Attributes h))
-  : forall (tup tup' : Tuple),
-      {tupleAgree tup tup' attrlist} + {~tupleAgree tup tup' attrlist}.
-  Proof.
-  Admitted.
+Fixpoint Tuple_Agree_dec
+         (h : Heading)
+         (h_dec_eq : decideable_Heading_Domain h)
+         (attrlist : list (Attributes h))
+: forall (tup tup' : Tuple),
+    {tupleAgree tup tup' attrlist} + {~tupleAgree tup tup' attrlist}.
+Proof.
+Admitted.
 
-  Fixpoint Check_List_Prop {A}
-           (cond : A -> bool)
-           (l : list A)
-  : bool :=
-    match l with
-        | [] => true
-        | a :: l' => if (cond a) then
-                          Check_List_Prop cond l'
-                        else false
-    end.
+Fixpoint Check_List_Prop {A}
+         (cond : A -> bool)
+         (l : list A)
+: bool :=
+  match l with
+    | [] => true
+    | a :: l' => if (cond a) then
+                   Check_List_Prop cond l'
+                 else false
+  end.
 
-  Definition In_List_Key
+Definition In_List_Key
            (h : Heading)
            (h_dec_eq : decideable_Heading_Domain h)
            (attrlist : list (Attributes h))
            (tup : Tuple)
            (l : list Tuple) :=
-    Check_List_Prop (fun tup' =>
-                       if (Tuple_Agree_dec h_dec_eq attrlist tup tup')
-                       then true
-                       else false) l.
+  Check_List_Prop (fun tup' =>
+                     if (Tuple_Agree_dec h_dec_eq attrlist tup tup')
+                     then true
+                     else false) l.
 
-  Lemma refine_unused_key_check
-  : forall (h : Heading)
-           (h_dec_eq : decideable_Heading_Domain h)
-           (attrlist attrlist' : list (Attributes h))
-           (tup : Tuple)
-           (rel : Ensemble Tuple)
-           (l : list Tuple),
-      EnsembleListEquivalence rel l
-      -> refine {b | decides b
-                             (forall tup' : Tuple,
-                                rel tup' ->
-                                tupleAgree tup tup' attrlist' ->
-                                tupleAgree tup tup' attrlist)}
-                (ret (In_List_Key h_dec_eq attrlist tup l)).
-  Admitted.
+Lemma refine_unused_key_check
+: forall (h : Heading)
+         (h_dec_eq : decideable_Heading_Domain h)
+         (attrlist attrlist' : list (Attributes h))
+         (tup : Tuple)
+         (rel : Ensemble Tuple)
+         (l : list Tuple),
+    EnsembleListEquivalence rel l
+    -> refine {b | decides b
+                           (forall tup' : Tuple,
+                              rel tup' ->
+                              tupleAgree tup tup' attrlist' ->
+                              tupleAgree tup tup' attrlist)}
+              (ret (In_List_Key h_dec_eq attrlist tup l)).
+Admitted.
 
-  Lemma refine_unused_key_check'
-  : forall (h : Heading)
-           (h_dec_eq : decideable_Heading_Domain h)
-           (attrlist attrlist' : list (Attributes h))
-           (tup : Tuple)
-           (rel : Ensemble Tuple)
-           (l : list Tuple),
-      EnsembleListEquivalence rel l
-      -> refine {b | decides b
-                             (forall tup' : Tuple,
-                                rel tup' ->
-                                tupleAgree tup' tup attrlist' ->
-                                tupleAgree tup' tup attrlist)}
-                (ret (In_List_Key h_dec_eq attrlist tup l)).
-  Admitted.
+Lemma refine_unused_key_check'
+: forall (h : Heading)
+         (h_dec_eq : decideable_Heading_Domain h)
+         (attrlist attrlist' : list (Attributes h))
+         (tup : Tuple)
+         (rel : Ensemble Tuple)
+         (l : list Tuple),
+    EnsembleListEquivalence rel l
+    -> refine {b | decides b
+                           (forall tup' : Tuple,
+                              rel tup' ->
+                              tupleAgree tup' tup attrlist' ->
+                              tupleAgree tup' tup attrlist)}
+              (ret (In_List_Key h_dec_eq attrlist tup l)).
+Admitted.
 
-  Lemma refine_foreign_key_check
-  : forall (h : Heading)
-           (rel : Ensemble Tuple)
-           (l : list Tuple)
-           (P : Ensemble Tuple)
-           (cond : Tuple -> bool),
-      EnsembleListEquivalence rel l
-      -> refine {b  |
-                 decides b
-                         (exists tup' : @Tuple h,
-                            rel tup' /\
-                            P tup')}
-                (ret (Check_List_Prop cond l)).
-    Admitted.
+Lemma refine_foreign_key_check
+      (h : Heading)
+      (rel : Ensemble Tuple)
+      (l : list Tuple)
+      (P : Ensemble Tuple)
+      (P_dec : DecideableWhereClause P)
+: EnsembleListEquivalence rel l
+    -> refine {b  |
+               decides b
+                       (exists tup' : @Tuple h,
+                          rel tup' /\
+                          P tup')}
+              (ret (Check_List_Prop cond l)).
+Admitted.
 
-      Add Parametric Morphism {A: Type} (b : bool):
-        (If_Then_Else b)
-          with signature (
-            @refine A ==> @refine A ==> refine)
-            as refine_refine_if.
-      Proof.
-        unfold refine, If_Then_Else; intros.
-        destruct b; eauto.
-      Qed.
+Add Parametric Morphism {A: Type} (b : bool):
+  (If_Then_Else b)
+    with signature (
+      @refine A ==> @refine A ==> refine)
+      as refine_refine_if.
+Proof.
+  unfold refine, If_Then_Else; intros.
+  destruct b; eauto.
+Qed.
+
+Lemma ImplementListInsert_eq qsSchema Ridx
+      (tup : Tuple)
+      (or : UnConstrQueryStructure qsSchema)
+      (nr : list (Tuple))
+:
+  EnsembleListEquivalence (GetUnConstrRelation or Ridx) nr
+  -> refine
+       {a |
+        EnsembleListEquivalence
+          (GetUnConstrRelation
+             (UpdateUnConstrRelation qsSchema or Ridx
+                                     (RelationInsert tup (GetUnConstrRelation or Ridx))) Ridx) a}
+       (ret (tup :: nr)).
+Proof.
+  unfold refine; intros; inversion_by computes_to_inv; subst; constructor.
+  unfold GetUnConstrRelation, UpdateUnConstrRelation in *.
+  rewrite ith_replace_BoundIndex_eq.
+  unfold EnsembleListEquivalence, RelationInsert, In, List.In in *; split; intuition.
+  right; apply H; auto.
+  right; apply H; auto.
+Qed.
+
+Lemma ImplementListInsert_neq qsSchema Ridx Ridx'
+      (tup : Tuple)
+      (or : UnConstrQueryStructure qsSchema)
+      (nr : list (Tuple))
+:
+  Ridx <> Ridx'
+  -> EnsembleListEquivalence (GetUnConstrRelation or Ridx) nr
+  -> refine
+       {a |
+        EnsembleListEquivalence
+          (GetUnConstrRelation
+             (UpdateUnConstrRelation qsSchema or Ridx'
+                                     (RelationInsert tup (GetUnConstrRelation or Ridx'))) Ridx) a}
+       (ret nr).
+Proof.
+  unfold refine; intros; inversion_by computes_to_inv; subst; constructor.
+  unfold GetUnConstrRelation, UpdateUnConstrRelation in *.
+  rewrite ith_replace_BoundIndex_neq; eauto using string_dec.
+Qed.
+
+Tactic Notation "implement" "insert" "for" "lists" :=
+  repeat (progress
+            (try (setoid_rewrite ImplementListInsert_eq; eauto;
+                  simplify with monad laws);
+             try (setoid_rewrite ImplementListInsert_neq;
+                  eauto; simplify with monad laws);
+             try (match goal with
+                    | |- context [ (GetUnConstrRelation _ ?Ridx) ] =>
+                      setoid_rewrite (@ImplementListInsert_neq _ Ridx)
+                  end; eauto; simplify with monad laws)));
+  try reflexivity.
