ADTExamples/QueryStructure/ListQueryRefinements.v
@@ -6,130 +6,138 @@ Require Import ProcessScheduler.AdditionalLemmas SetEq.
 
 Lemma refine_SetEq_self {A} :
   forall l : list A,
-      refine {l' | SetEq l' l}%comp
-             (ret l).
+    refine {l' | SetEq l' l}%comp
+           (ret l).
 Proof.
   unfold SetEq, refine; intros; inversion_by computes_to_inv.
-    econstructor; subst; split; eauto.
+  econstructor; subst; split; eauto.
 Qed.
 
 Lemma Equivalent_In_EnsembleListEquivalence {A}
-        (qs : QueryStructureHint) (R : _)
-        (l : list _)
-        bod
+      (qs : QueryStructureHint) (R : _)
+      (l : list _)
+      bod
 : EnsembleListEquivalence (GetRelation qsHint R) l ->
   Equivalent_Ensembles
     (@Query_In qs A R bod)
     (fun a => exists tup, List.In tup l /\ bod tup a).
 Proof.
-    split; intros; unfold In in *.
-    destruct H0; eexists; intuition; eauto.
-    eapply H; eauto.
-    destruct H0; intuition; eexists; split; eauto.
-    eapply H; eauto.
+  split; intros; unfold In in *.
+  destruct H0; eexists; intuition; eauto.
+  eapply H; eauto.
+  destruct H0; intuition; eexists; split; eauto.
+  eapply H; eauto.
 Qed.
 
-  Definition Join_Lists {A B}
-             (l : list A)
-             (l' : list B)
-  : list (A * B) :=
-    fold_left (@app _) (map (fun a => map (fun b => (a, b)) l') l) nil.
-
-  Lemma In_fold_left_app {A}
-  : forall (l : list (list A))
-           (l'' : list A)
-           (a : A),
-      List.In a (fold_left (@app _) l l'') <->
-      (List.In a l'' \/ (exists l', List.In l' l /\ List.In a l')).
-  Proof.
-    induction l; simpl; intuition.
-    destruct_ex; intuition.
-    destruct (proj1 (IHl _ _) H).
-    apply in_app_or in H0; intuition; eauto.
-    destruct_ex; intuition; eauto.
-    eapply IHl; eauto using in_or_app.
-    destruct_ex; intuition; subst; eauto.
-    eapply IHl; eauto using in_or_app.
-    eapply IHl; eauto using in_or_app.
-  Qed.
-
-  Lemma In_Join_Lists {A B}
-  : forall (l : list A)
+Definition Join_Lists {A B}
+           (l : list A)
            (l' : list B)
-           (a : A)
-           (b : B),
-      List.In (a, b) (Join_Lists l l') <->
-      (List.In a l /\ List.In b l').
-  Proof.
-    unfold Join_Lists; split; intros.
-    apply In_fold_left_app in H; simpl in *; intuition;
-    destruct_ex; intuition;
-    apply in_map_iff in H0; destruct_ex; intuition; subst;
-    apply in_map_iff in H1; destruct_ex; intuition; subst;
-    simpl; congruence.
-    intuition.
-    apply In_fold_left_app; right.
-    exists (map (fun b : B => (a, b)) l'); split;
-    apply in_map_iff; eexists; intuition; eauto.
-  Qed.
+: list (A * B) :=
+  fold_left (@app _) (map (fun a => map (fun b => (a, b)) l') l) nil.
 
-  Lemma Equivalent_Join_Lists {A B}
-        (qs : QueryStructureHint) (R : _)
-        (l : list B)
-        (l' : list _)
-        bod
-  : EnsembleListEquivalence (GetRelation qsHint R) l' ->
-    Equivalent_Ensembles
-      (fun a => exists b, List.In b l /\
-                            (@Query_In qs A R (bod b) a))
-      (fun a => exists b, List.In b (Join_Lists l l') /\
-                          (bod (fst b) (snd b) a)).
-  Proof.
-    split; intros; unfold In in *.
-    - destruct H0; intuition; destruct H2; eexists; intuition; eauto.
-      unfold EnsembleListEquivalence in H.
-      apply In_Join_Lists; split; eauto.
-      eapply H; unfold In; apply H2.
-      simpl; auto.
-    - destruct_ex; intuition; destruct x; eexists; intuition.
-      eapply (In_Join_Lists l l'); eauto.
-      unfold Query_In; eexists; intuition; eauto.
-      apply H; eapply (In_Join_Lists l l'); eauto.
-  Qed.
+Lemma In_fold_left_app {A}
+: forall (l : list (list A))
+         (l'' : list A)
+         (a : A),
+    List.In a (fold_left (@app _) l l'') <->
+    (List.In a l'' \/ (exists l', List.In l' l /\ List.In a l')).
+Proof.
+  induction l; simpl; intuition.
+  destruct_ex; intuition.
+  destruct (proj1 (IHl _ _) H).
+  apply in_app_or in H0; intuition; eauto.
+  destruct_ex; intuition; eauto.
+  eapply IHl; eauto using in_or_app.
+  destruct_ex; intuition; subst; eauto.
+  eapply IHl; eauto using in_or_app.
+  eapply IHl; eauto using in_or_app.
+Qed.
 
-  Lemma Equivalent_List_In_Where {A B}
-        (l : list B)
-        (P : Ensemble B)
-        (bod : B -> Ensemble A)
-        (cond : B -> bool)
-        : (forall a, cond a = true <-> P a)
-          ->
-    Equivalent_Ensembles
-      (fun a : A => exists b, List.In b l /\ Query_Where (P b) (bod b) a)
-      (fun a : A => exists b, List.In b (filter cond l) /\ (bod b) a)
-  .
-  Proof.
-    split; intros; unfold In, Query_Where in *.
-    destruct H0; eexists; intuition; eauto.
-    eapply filter_In; split; eauto.
-    eapply H; eauto.
-    destruct H0; intuition; eexists; split; eauto.
-    eapply filter_In; eauto.
-    intuition; eauto using filter_In.
-    eapply H; eapply filter_In; eauto.
-  Qed.
+Lemma In_Join_Lists {A B}
+: forall (l : list A)
+         (l' : list B)
+         (a : A)
+         (b : B),
+    List.In (a, b) (Join_Lists l l') <->
+    (List.In a l /\ List.In b l').
+Proof.
+  unfold Join_Lists; split; intros.
+  apply In_fold_left_app in H; simpl in *; intuition;
+  destruct_ex; intuition;
+  apply in_map_iff in H0; destruct_ex; intuition; subst;
+  apply in_map_iff in H1; destruct_ex; intuition; subst;
+  simpl; congruence.
+  intuition.
+  apply In_fold_left_app; right.
+  exists (map (fun b : B => (a, b)) l'); split;
+  apply in_map_iff; eexists; intuition; eauto.
+Qed.
 
-  Lemma refine_For_List_Return {A B}
-        (l : list B)
-        (extract : B -> A)
-  : refine
-      (For (fun a : A =>
-              exists b : B,
-                List.In b l /\ Return (extract b) a))%QuerySpec
-      (ret (map extract l)).
-  Proof.
-    unfold refine; intros; inversion_by computes_to_inv; subst.
-    econstructor; unfold In, Query_Return; split; intros.
-    eapply in_map_iff in H; destruct_ex; intuition; eauto.
-    eapply in_map_iff; destruct_ex; intuition; eauto.
-  Qed.
+Lemma Equivalent_Join_Lists {A B}
+      (qs : QueryStructureHint) (R : _)
+      (l : list B)
+      (l' : list _)
+      bod
+: EnsembleListEquivalence (GetRelation qsHint R) l' ->
+  Equivalent_Ensembles
+    (fun a => exists b, List.In b l /\
+                        (@Query_In qs A R (bod b) a))
+    (fun a => exists b, List.In b (Join_Lists l l') /\
+                        (bod (fst b) (snd b) a)).
+Proof.
+  split; intros; unfold In in *.
+  - destruct H0; intuition; destruct H2; eexists; intuition; eauto.
+    unfold EnsembleListEquivalence in H.
+    apply In_Join_Lists; split; eauto.
+    eapply H; unfold In; apply H2.
+    simpl; auto.
+  - destruct_ex; intuition; destruct x; eexists; intuition.
+    eapply (In_Join_Lists l l'); eauto.
+    unfold Query_In; eexists; intuition; eauto.
+    apply H; eapply (In_Join_Lists l l'); eauto.
+Qed.
+
+Lemma Equivalent_List_In_Where {A B : Type}
+      (l : list B)
+      (P : Ensemble B)
+      (bod : B -> Ensemble A)
+      (P_dec : DecideableWhereClause P)
+:
+  Equivalent_Ensembles
+    (fun a : A => exists b, List.In b l /\ Query_Where (P b) (bod b) a)
+    (fun a : A => exists b, List.In b (filter cond l) /\ (bod b) a)
+.
+Proof.
+  destruct P_dec; split; intros; unfold In, Query_Where in *.
+  destruct H; eexists; intuition; eauto.
+  eapply filter_In; split; eauto.
+  eapply cond_dec; eauto.
+  destruct H; intuition; eexists; split; eauto.
+  eapply filter_In; eauto.
+  intuition; eauto using filter_In.
+  eapply cond_dec; eapply filter_In; eauto.
+Qed.
+
+Lemma refine_For_List_Return {A B}
+      (l : list B)
+      (extract : B -> A)
+: refine
+    (For (fun a : A =>
+            exists b : B,
+              List.In b l /\ Return (extract b) a))%QuerySpec
+    (ret (map extract l)).
+Proof.
+  unfold refine; intros; inversion_by computes_to_inv; subst.
+  econstructor; unfold In, Query_Return; split; intros.
+  eapply in_map_iff in H; destruct_ex; intuition; eauto.
+  eapply in_map_iff; destruct_ex; intuition; eauto.
+Qed.
+
+Tactic Notation "implement" "queries" "for" "lists" :=
+  unfold DropQSConstraints_SiR in *; subst;
+  repeat rewrite GetRelDropConstraints in *; subst; split_and;
+  repeat (progress
+            (try (setoid_rewrite Equivalent_In_EnsembleListEquivalence; simpl; eauto);
+             try (setoid_rewrite Equivalent_List_In_Where with (P_dec := _); simpl);
+             try (setoid_rewrite Equivalent_Join_Lists; eauto)));
+  setoid_rewrite refine_For_List_Return; simplify with monad laws.
