ADTRefinement/GeneralBuildADTRefinements.v
@@ -330,7 +330,8 @@ Tactic Notation "hone'" "mutator" constr(mutIdx) :=
                                 _
                ));
       [ intros; try (apply refine_pick_forall_Prop with
-                     (P := fun r_n n r_o => _); intros) |
+                     (P := fun r_n n r_o => _); intros);
+        set_evars; simpl in *; subst |
           cbv beta in *; simpl in *;
           cbv beta delta [replace_BoundedIndex replace_Index] in *;
           simpl in *].
@@ -371,8 +372,10 @@ Tactic Notation "hone'" "mutator" constr(mutIdx) :=
                                  |}
                                  _
                                 ));
-          [ intros; try (apply refine_pick_forall_Prop with
-                         (P := fun r_n n r_o => _); intros) |
+      [ intros; repeat (progress (try rewrite refine_pick_computes_to;
+                                  try apply refine_pick_forall_Prop with
+                                  (P := fun _ _ _ => _); intros));
+        set_evars; simpl in *; subst |
             cbv beta in *; simpl in *;
             cbv beta delta [replace_BoundedIndex replace_Index] in *;
             simpl in *].
